proof/infoflow/FinalCaps.thy
@@ -3075,7 +3075,7 @@ lemma handle_interrupt_silc_inv:
   "\<lbrace>silc_inv aag st\<rbrace> handle_interrupt irq \<lbrace>\<lambda>_. silc_inv aag st\<rbrace>"
   unfolding handle_interrupt_def
   apply (rule hoare_if)  
-  apply(wp | wpc | simp | wp_once hoare_drop_imps)+
+  apply(wp | wpc | simp add: handle_reserved_irq_def | wp_once hoare_drop_imps)+
   done
 
 lemma handle_vm_fault_silc_inv:
